\documentclass[12pt]{article}
 \usepackage[margin=1in]{geometry} 
\usepackage{amsmath,amsthm,amssymb,amsfonts}
\usepackage{stackengine}
 
\newcommand{\longdiv}[2]{$#1\overline{\smash{)}#2}$}
\newcommand{\N}{\mathbb{N}}
\newcommand{\Z}{\mathbb{Z}}
 
\newenvironment{problem}[2][Problem]{\begin{trivlist}
\item[\hskip \labelsep {\bfseries #1}\hskip \labelsep {\bfseries #2.}]}{\end{trivlist}}

\title{Pg. 221-223, #1-5, 14-28 even, 53, 55}
\author{Mia Jones}
\date{November 26 2018}

\begin{document}

\maketitle


\begin{problem}{1}
To add fractions with different denominators, first rewrite the fraction using the \boxed{\text{LCD.}}
\end{problem}

\begin{problem}{2}
$\frac{1}{10} + \frac{8}{10} = \boxed{\frac{9}{10}}.$
\end{problem}

\begin{problem}{3}
$\frac{4}{7} + \frac{5}{7} = \frac{9}{7} = \boxed{1 \frac{2}{7}}.$
\end{problem}

\begin{problem}{4}
$\frac{5}{7} + \frac{1}{7} = \boxed{\frac{6}{7}}.$
\end{problem}

\begin{problem}{5}
$\frac{9}{20} + \frac{7}{20} = \frac{16}{20} = \boxed{\frac{4}{5}}.$
\end{problem}

\begin{problem}{14}
$\frac{3}{5} + \frac{7}{10} = \frac{6}{10} + \frac{7}{10} = \frac{13}{10} = \boxed{1 \frac{3}{10}}.$
\end{problem}

\begin{problem}{16}
$\frac{2}{3} + \frac{1}{4} = \frac{8}{12} + \frac{3}{12} = \boxed{\frac{11}{12}}.$
\end{problem}

\begin{problem}{18}
$\frac{1}{6} + \frac{3}{4} = \frac{2}{12} + \frac{9}{12} = \boxed{\frac{11}{12}}.$
\end{problem}

\begin{problem}{20}
$\frac{11}{12} - \frac{3}{4} = \frac{11}{12} - \frac{9}{12} = \frac{2}{12} = \boxed{\frac{1}{6}}.$
\end{problem}

\begin{problem}{22}
$\frac{3}{8} - \frac{1}{3} = \frac{9}{24} = \frac{8}{24} = \boxed{\frac{1}{24}}.$
\end{problem}

\begin{problem}{24}
$\frac{3}{4} - \frac{1}{6} = \frac{9}{12} - \frac{2}{12} = \boxed{\frac{7}{12}}.$
\end{problem}

\begin{problem}{26}
$\frac{3}{8} + \frac{5}{16} + \frac{7}{8} = \frac{6}{16} + \frac{5}{16}  \frac{14}{16} = \frac{25}{16} = \boxed{1 \frac{9}{16}}.$
\end{problem}

\begin{problem}{28}
$\frac{2}{3} + \frac{3}{4} - \frac{2}{5} = \frac{40}{60} + \frac{45}{60} - \frac{24}{60} = \frac{85}{60} - \frac{24}{60} = \frac{61}{60} = \boxed{1 \frac{1}{60}}.$
\end{problem}

\begin{problem}{53}
$\frac{3}{4} + \frac{5}{12} = \frac{9}{12} + \frac{5}{12} = \frac{14}{12} = \boxed{1 \frac{1}{6}}$.
\end{problem}

\begin{problem}{55}
$\frac{1}{2} - \frac{1}{8} = \frac{4}{8} - \frac{1}{8} = \boxed{\frac{3}{8}}.$
\end{problem}

\end{document}